\begin{thm}
  For a given network $N(S,T)$ with sensors $s\in S$ and targets $t\in T$, there exists an equivalent hypergraph $G(V,E)$ such that any solution to the target coverage problem (TC) in $N$ is an edge cover (EC) in $G$, and any edge cover of $G$ is a target cover for $N$.
\label{thm:equiv}
\end{thm}
\begin{proof}[Proof of Theorem~\ref{thm:equiv}]
\begin{prop}
For $N(S,T)$, identify $t \in T | t_i = s \in S $ such that $s$ covers $t$. That is, if sensors $s_1, s_4, s_7$ are all of the sensors that cover $t_3$, $t_3 = \{s_1, s_4, s_5\}$. \label{prp:network}
\end{prop}
\begin{prop}To construct the equivalent hypergraph $G(V,E)$, define $f:S\to V$ and $g:T\to E$ as bijective functions $f(s)$ and $g(t)$, that is, every sensor and every target should have a corresponding vertex and edge, and these are the only vertexes and edges in $G$. We impose a further restriction that $ s_j \in t_i \implies f(s_j) \in g(t_i)$. 
\label{prp:graph}
\end{prop}

To be shown: if $S' \subset S$ is a solution for target coverage in $N$, $f(S')$ is an edge cover of $G$. 

We proceed by direct proof. Let us define $S'\subset S$ such that $S'$ is a target cover of $N$. If $S'$ is a target cover, we know that 
\begin{equation}
\forall t \in T, \exists s \in t | s \in S'
\label{eqn:tcover}
\end{equation}
That is, for every target, there is a sensor in $S'$ that covers that target.

We also know that there exists an equivalent edge in $G$ for each target, defined as $g(t)$. We rewrite equation~\ref{eqn:tcover} to include proposition~\ref{prp:graph},
\begin{equation}
\forall t \in T, \exists s \in t | s \in S' \land f(s) \in g(t)
\label{eqn:extcover}
\end{equation}

Since the range of $g$ is comprehensive of $E$, this implies that for all edges,
\begin{equation}
\forall e \in E, \exists s \in S' | f(s) \in e
\end{equation}
Therefore, is we apply $f(s)$ to every $s \in S'$, we will create a vertex set $V'$ such that
\begin{equation}
\forall e \in E, \exists v \in V' | v \in e
\label{eqn:vcover}
\end{equation}
Equation~\ref{eqn:vcover} describes a vertex cover of $G$, which is what we wanted to find.

The second part of the theorem follows from the definition of bijection. 
\end{proof}